added a new test but it goes all the way to the swap

test.ml
@@ -4,7 +4,7 @@ let rec gen_bin_list n =
   if 0 = n
   then []
   else (if Random.int 2 = 0 then O else S O)::gen_bin_list (n - 1)
-  
+
 let test_aes =
   let l = gen_bin_list (12 * 128) in
   prog_sem default_arch prog_aes None [CoIR (DirB, l, None)]
@@ -12,4 +12,3 @@ let test_aes =
 let () = match test_aes with
   | None -> print_endline "Failure AES"
   | Some _ -> print_endline "Success AES"
-
