src/usuba_AST.v
@@ -1,11 +1,8 @@
 Require Import String.
-Require Import Coq.Lists.List.
-Require Import Coq.FSets.FMapAVL.
-Require Import Coq.Structures.OrderedTypeEx.
-From mathcomp Require Import all_ssreflect.
-Module Import NatMap := FMapList.Make(String_as_OT).
-From Coq Require Import Program Arith.
-From Coq Require Recdef.
+Require Import List.
+Require Import ZArith.
+Require Import Bool.
+From mathcomp Require Import seq ssrnat.
 
 Inductive ident :=
     | Id_s : string -> ident
@@ -50,36 +47,24 @@ Definition shift_op_size (x : shift_op) : nat := 1.
 
 (** ARITHMETIC EXPRESSIONS **)
 
-Inductive arith_expr :=
-    | Const_e : nat -> arith_expr
+Inductive arith_expr : Type :=
+    | Const_e : Z -> arith_expr
     | Var_e : ident -> arith_expr
     | Op_e : arith_op -> arith_expr -> arith_expr -> arith_expr.
 Scheme Equality for arith_expr.
-Function arith_expr_size (e : arith_expr) :=
+
+Fixpoint arith_expr_size (e : arith_expr) :=
     match e with
     | Const_e _ => 1
     | Var_e _ => 1
     | Op_e op e1 e2 => 1 + arith_op_size op + arith_expr_size e1 + arith_expr_size e2
     end.
-Function arith_expr_list_size (el : list arith_expr) :=
+
+Fixpoint arith_expr_list_size (el : seq arith_expr) :=
     match el with
     | nil => 0
     | h :: t => 1 + arith_expr_size h + arith_expr_list_size t
     end.
-
-Definition alpha_equal_ident (ctxt :  NatMap.t ident) (id1 : ident) (id2 : ident) : bool :=
-    ident_beq id1 id2.
-
-Fixpoint alpha_equal_arith_expr (ctxt :  NatMap.t ident) (ae1 : arith_expr) (ae2 : arith_expr) : bool :=
-    match (ae1, ae2) with
-        | (Const_e i1, Const_e i2) => i1 =? i2
-        | (Var_e id1, Var_e id2) => alpha_equal_ident ctxt id1 id2
-        | (Op_e op1 ae11 ae12, Op_e op2 ae21 ae22) =>
-            arith_op_beq op1 op2
-            && alpha_equal_arith_expr ctxt ae11 ae21
-            && alpha_equal_arith_expr ctxt ae12 ae22
-        | _ => false
-        end.
 
 (** TYPES *)
 
@@ -91,21 +76,21 @@ Inductive dir :=
     | Varslice : ident -> dir
     | Mslice : nat -> dir.
 Scheme Equality for dir.
-Function dir_size (d : dir) := 1.
+Definition dir_size (d : dir) := 1.
 
 Inductive mtyp :=
     | Mint : nat -> mtyp
     | Mnat : mtyp
     | Mvar : ident -> mtyp.
 Scheme Equality for mtyp.
-Function mtyp_size (m : mtyp) := 1. 
+Definition mtyp_size (m : mtyp) := 1. 
 
 Inductive typ :=
     | Nat : typ
     | Uint : dir -> mtyp -> nat -> typ
     | Array : typ -> arith_expr -> typ.
 Scheme Equality for typ.
-Function typ_size (t : typ) :=
+Fixpoint typ_size (t : typ) :=
     match t with
     | Nat => 1
     | Uint d m n => 1 + dir_size d + mtyp_size m + n
@@ -118,9 +103,9 @@ Inductive var :=
     | Var : ident -> var
     | Index : var -> arith_expr -> var
     | Range : var -> arith_expr -> arith_expr -> var
-    | Slice : var -> list arith_expr -> var.
+    | Slice : var -> seq arith_expr -> var.
 
-Function var_size (v : var) :=
+Fixpoint var_size (v : var) :=
     match v with
     | Var _ => 1
     | Index v e => 1 + var_size v + arith_expr_size e
@@ -128,33 +113,17 @@ Function var_size (v : var) :=
     | Slice v el => 1 + var_size v + arith_expr_list_size el
     end.
 
-Function list_var_size (v : list var) :=
+Fixpoint list_var_size (v : seq var) :=
     match v with
     | nil => 0
     | hd::tl => 1 + var_size hd + list_var_size tl
     end.
 
-Fixpoint list_eq {A} (eq : A -> A -> bool) (l1 : list A) (l2 : list A) :=
+Fixpoint list_eq {A} (eq : A -> A -> bool) (l1 : seq A) (l2 : seq A) :=
     match (l1, l2) with
     | (nil, nil) => true
     | (nil, _) | (_, nil) => false
     | (h1 :: t1, h2 :: t2) => eq h1 h2 && list_eq eq t1 t2
-    end.
-
-Fixpoint alpha_equal_var (ctxt :  NatMap.t ident) (v1 : var) (v2 : var) :=
-    match (v1, v2) with
-    | (Var id1, Var id2) => alpha_equal_ident ctxt id1 id2
-    | (Index v1 ae1, Index v2 ae2) =>
-        alpha_equal_var ctxt v1 v2
-        && alpha_equal_arith_expr ctxt ae1 ae2
-    | (Range v1 ae11 ae12, Range v2 ae21 ae22) =>
-        alpha_equal_var ctxt v1 v2
-        && alpha_equal_arith_expr ctxt ae11 ae21
-        && alpha_equal_arith_expr ctxt ae12 ae22
-    | (Slice v1 ael1, Slice v2 ael2) =>
-        alpha_equal_var ctxt v1 v2
-        && list_eq (alpha_equal_arith_expr ctxt) ael1 ael2
-    | _ => false
     end.
 
 (** EXPRESSIONS *)
@@ -167,7 +136,7 @@ Inductive expr :=
   | Log : log_op -> expr -> expr -> expr
   | Arith : arith_op -> expr -> expr -> expr
   | Shift : shift_op -> expr -> arith_expr -> expr
-  | Shuffle : var -> list nat -> expr
+  | Shuffle : var -> seq nat -> expr
   | Bitmask : expr -> arith_expr -> expr
   | Pack : expr -> expr -> option typ -> expr
   | Fun : ident -> expr_list -> expr
@@ -179,7 +148,7 @@ with expr_list :=
 Scheme expr_find := Induction for expr Sort Prop
 with expr_list_find := Induction for expr_list Sort Prop.
   
-Function expr_size (e : expr) : nat :=
+Fixpoint expr_size (e : expr) : nat :=
     match e with
     | Const n None => 1
     | Const n (Some t) => 1 + typ_size t
@@ -202,48 +171,12 @@ with expr_list_size (el : expr_list) : nat :=
     | ECons h t => 1 + expr_size h + expr_list_size t
     end.
 
-Function alpha_equal_expr (ctxt :  NatMap.t ident) (e1 : expr) (e2 : expr) : bool :=
-    match (e1, e2) with
-    | (Const i1 t1, Const i2 t2) => (i1 =? i2) && t1 == t2
-    | (ExpVar v1, ExpVar v2) => alpha_equal_var ctxt v1 v2
-    | (Tuple el1, Tuple el2) => alpha_equal_expr_list ctxt el1 el2
-    | (Not e1, Not e2) => alpha_equal_expr ctxt e1 e2
-    | (Log op1 e11 e12, Log op2 e21 e22) =>
-        log_op_beq op1 op2 && alpha_equal_expr ctxt e11 e21 && alpha_equal_expr ctxt e12 e22
-    | (Arith op1 e11 e12, Arith op2 e21 e22) =>
-        arith_op_beq op1 op2 && alpha_equal_expr ctxt e11 e21 && alpha_equal_expr ctxt e12 e22
-    | (Shift op1 e1 ae1, Shift op2 e2 ae2) =>
-        shift_op_beq op1 op2 && alpha_equal_expr ctxt e1 e2
-        && alpha_equal_arith_expr ctxt ae1 ae2
-    | (Shuffle v1 il1, Shuffle v2 il2) =>
-        alpha_equal_var ctxt v1 v2 && list_eq Nat.eqb il1 il2
-    | (Bitmask e1 ae1, Bitmask e2 ae2) =>
-        alpha_equal_expr ctxt e1 e2 && alpha_equal_arith_expr ctxt ae1 ae2
-    | (Pack e11 e12 t1, Pack e21 e22 t2) =>
-        alpha_equal_expr ctxt e11 e21 && alpha_equal_expr ctxt e12 e22 && t1 == t2
-    | (Fun id1 el1, Fun id2 el2) =>
-        alpha_equal_ident ctxt id1 id2 && alpha_equal_expr_list ctxt el1 el2
-    | (Fun_v id1 ae1 el1, Fun_v id2 ae2 el2) =>
-        alpha_equal_ident ctxt id1 id2
-        && alpha_equal_arith_expr ctxt ae1 ae2
-        && alpha_equal_expr_list ctxt el1 el2
-    | _ => false
-    end
-with alpha_equal_expr_list (ctxt :  NatMap.t ident) (el1 : expr_list) (el2 : expr_list) : bool :=
-    match (el1, el2) with
-        | (Enil, Enil) => true
-        | (Enil, _) | (_, Enil) => false
-        | (ECons e1 t1, ECons e2 t2) =>
-            alpha_equal_expr ctxt e1 e2
-            && alpha_equal_expr_list ctxt t1 t2
-    end.
-
 Inductive stmt_opt :=
     Unroll | No_unrool | Pipelined | Safe_exit.
 
 Inductive deq :=
-    | Eqn : list var -> expr -> bool -> deq
-    | Loop : ident -> arith_expr -> arith_expr -> list_deq -> list stmt_opt -> deq
+    | Eqn : seq var -> expr -> bool -> deq
+    | Loop : ident -> arith_expr -> arith_expr -> list_deq -> seq stmt_opt -> deq
 with list_deq :=
     | Dnil
     | Dcons : deq -> list_deq -> list_deq.
@@ -251,7 +184,7 @@ with list_deq :=
 Scheme deq_find := Induction for deq Sort Prop
 with list_deq_find := Induction for list_deq Sort Prop.
 
-Function deq_size deq : nat :=
+Fixpoint deq_size deq : nat :=
     match deq with
     | Eqn v e b => 1 + list_var_size v + expr_size e
     | Loop id ae1 ae2 dl stmt => 1 + arith_expr_size ae1 + arith_expr_size ae2 +
@@ -267,15 +200,15 @@ Inductive var_d_opt := Pconst | PlazyLift.
 Record var_d := {
     VD_ID : ident;
     VD_TYP : typ;
-    VD_OPTS : list var_d_opt;
+    VD_OPTS : seq var_d_opt;
 }.
 
-Definition p := list var_d.
+Definition p := seq var_d.
 
 Inductive def_i :=
     | Single : p -> list_deq -> def_i
-    | Perm : list nat -> def_i
-    | Table : list nat -> def_i
+    | Perm : seq nat -> def_i
+    | Table : seq nat -> def_i
     | Multiple : list_def_i -> def_i
 with list_def_i :=
     | LDnil
@@ -298,4 +231,4 @@ Inductive def_or_inc :=
     | Def : def -> def_or_inc
     | Inc : string -> def_or_inc.
 
-Definition prog := list def.
+Definition prog := seq def.
