src/arch.v
@@ -1,0 +1,174 @@
+Require Import Bool.
+Require Import PeanoNat.
+Require Import List.
+From Usuba Require Import usuba_AST.
+
+Fixpoint take_n {A : Type} (nb : nat) (l : list A) : option (list A * list A) :=
+    match nb with
+    | 0 => Some (nil, l)
+    | S nb' => match l with
+        | nil => None
+        | hd :: tl =>
+            (s, e) <- take_n nb' tl;
+            Some (hd :: s, e)
+        end
+    end.
+
+Definition IntSize : Type := nat.
+Definition IntSize_beq := Nat.eqb.
+
+Definition IntSize_of_nat (n : nat) : option IntSize := Some n.
+
+Inductive dir :=
+    | DirH : IntSize -> dir
+    | DirV : IntSize -> dir
+    | DirB
+    | DirUnknow
+    | DirH_
+    | DirV_
+    | Dir_S : IntSize -> dir.
+Scheme Equality for dir.
+
+Fixpoint to_bits (len n : nat) : list bool :=
+    match len with
+    | 0 => nil
+    | S len' =>
+        (Nat.eqb (n mod 2) 1)::to_bits len' (n / 2)
+    end.
+
+Fixpoint from_bits (l : list bool) : nat :=
+    match l with
+    | nil => 0
+    | hd::tl => (if hd then 1 else 0) + 2 * from_bits tl
+    end.
+
+Definition chop (len n : nat) :=
+    from_bits (to_bits len n).
+
+Definition arith_wrapper {A : Type} (arch : dir -> bool) (op : nat -> A) (d : dir) : option A :=
+    if arch d
+    then
+        match d with
+        | DirV i | DirH i => Some (op i)
+        | DirB => Some (op 1)
+        | _ => None
+        end
+    else None.
+
+Fixpoint extend (len a : nat) : nat :=
+    match len with
+    | 0 => 1
+    | S len' => (a mod 2) + 2 * extend len' (a / 2)
+    end.
+
+Definition add_fun (len a b : nat) : nat := chop len (a + b).
+Definition sub_fun (len a b : nat) : nat := chop len ((extend len a) - b).
+Definition mod_fun (len a b : nat) : nat := chop len (a mod b).
+Definition div_fun (len a b : nat) : nat := chop len (a / b).
+Definition mul_fun (len a b : nat) : nat := chop len (a * b).
+
+Fixpoint map2 {A B C : Type} (f : A -> B -> C) l1 l2 : list C :=
+    match (l1, l2) with
+    | (nil, _) | (_, nil) => nil
+    | (h1::t1, h2::t2) => f h1 h2::map2 f t1 t2
+    end. 
+
+Definition lnot (len n : nat) : nat :=
+    from_bits (map negb (to_bits len n)).
+
+Definition land (len n1 n2 : nat) : nat :=
+    from_bits (map2 andb (to_bits len n1) (to_bits len n2)).
+
+Definition lor (len n1 n2 : nat) : nat :=
+    from_bits (map2 orb (to_bits len n1) (to_bits len n2)).
+
+Definition lxor (len n1 n2 : nat) : nat :=
+    from_bits (map2 xorb (to_bits len n1) (to_bits len n2)).
+
+Definition landn (len n1 n2 : nat) : nat :=
+    from_bits (map2 (fun a b => a && (negb b)) (to_bits len n1) (to_bits len n2)).
+
+Definition lshift (len s nb : nat) :=
+    match take_n (len - s) (to_bits len nb) with
+    | None => 0
+    | Some (l1, l2) => from_bits (map (fun _ => false) l2 ++ l1)
+    end.
+
+Goal
+    lshift 8 3 129 = 8.
+Proof. cbn. reflexivity. Qed.
+
+Definition rshift (len s nb : nat) :=
+    match take_n s (to_bits len nb) with
+    | None => 0
+    | Some (l1, l2) => from_bits (map (fun _ => false) l2 ++ l1)
+    end.
+
+Definition rashift (len s nb : nat) :=
+    let l := (to_bits len nb) in
+    let lst := last l false in
+    match take_n s l with
+    | None => 0
+    | Some (l1, l2) =>
+        from_bits (map (fun _ => lst) l2 ++ l1)
+    end.
+    
+Definition lrotate (len s nb : nat) :=
+    match take_n (len - s) (to_bits len nb) with
+    | None => 0
+    | Some (l1, l2) => from_bits (l2 ++ l1)
+    end.
+
+Definition rrotate (len s nb : nat) :=
+    match take_n s (to_bits len nb) with
+    | None => 0
+    | Some (l1, l2) => from_bits (l2 ++ l1)
+    end.
+
+Definition shift_wrapper (param : dir -> nat -> bool) (op : shift_op) (n : nat) (d : dir) (i : nat) : option nat :=
+    if param d n
+    then
+        let op := match op with
+            | Lshift => lshift
+            | Rshift => rshift
+            | RAshift => rashift
+            | Rrotate => rrotate
+            | Lrotate => lrotate
+        end in
+        match d with
+        | DirB => Some (op 1 n i)
+        | DirH len | DirV len => Some (op len n i)
+        | _ => None
+        end
+    else None.
+
+Record architecture : Type := {
+    IMPL_ARITH : dir -> bool;
+    IMPL_LOG : dir -> bool;
+    IMPL_SHIFT : dir -> nat -> bool;
+}.
+
+Definition default_arch : architecture := {|
+    IMPL_ARITH := fun d =>
+        match d with
+        | DirV 8 | DirV 16 | DirV 32 | DirV 64 => true
+        | _ => false
+        end;
+        
+    IMPL_LOG := fun d =>
+        match d with
+        | DirV _ | DirH _ | DirB => true
+        | _ => false
+        end;
+
+    IMPL_SHIFT := fun d s =>
+        match d with
+        | DirH 2 => Nat.ltb s 2
+        | DirH 4 => Nat.ltb s 4
+        | DirH 8 => Nat.ltb s 8
+        | DirV 16 | DirH 16 => Nat.ltb s 16
+        | DirV 32 | DirH 32 => Nat.ltb s 32
+        | DirV 64 | DirH 64 => Nat.ltb s 64
+        | _ => false
+        end
+|}.
