src/examples/ace_bitslice.v
@@ -1,0 +1,75 @@
+Require Import String List.
+From Usuba Require Import usuba_AST syntax arch.
+
+Definition simeck_box : string := "simeck_box".
+Definition ACE_step : string := "ACE_step".
+Definition ACE : string := "ACE".
+Definition rc : string := "rc".
+Definition Ar : string := "Ar".
+Definition Br : string := "Br".
+Definition Cr : string := "Cr".
+Definition Dr : string := "Dr".
+Definition Er : string := "Er".
+Definition A : string := "A".
+Definition B : string := "B".
+Definition C : string := "C".
+Definition D : string := "D".
+Definition E : string := "E".
+Definition RC : string := "RC".
+Definition SC : string := "SC".
+
+Definition node_f := node f args (x:u32) returns (y:u32) vars nil
+let
+    Var y :: nil <|- ((x <<< 5) & x) xor (x <<< 1)
+tel.
+
+Definition node_simeck_box := node simeck_box args input:u32x2, rc:u32 returns (output:u32x2)
+vars
+    (round:u32x2[9]) :: nil
+let
+    round[0] :: nil <|- input;
+
+    for i in 0 to 7 do
+      (round[i + 1] $ [0,1])%ua_var :: nil <|- [f @ [round[i][0]] xor round[i][1] xor 0xfffffffe xor ((rc >> i) & 1), round[i][0]]
+    done;
+
+    Var output :: nil <|- round[8]
+tel.
+
+Definition node_ACE_step := node ACE_step args A:u32x2,B:u32x2,C:u32x2,D:u32x2,E:u32x2,RC:u32[3],SC:u32[3]
+returns Ar:u32x2,Br:u32x2,Cr:u32x2,Dr:u32x2,Er:u32x2
+vars nil
+let
+    Var A :: nil <:- simeck_box @ [A,RC[0]];
+    Var C :: nil <:- simeck_box @ [C,RC[1]];
+    Var E :: nil <:- simeck_box @ [E,RC[2]];
+    Var B :: nil <:- B xor C xor [0,SC[0]] xor [0xffffffff,0xffffff00];
+    Var D :: nil <:- D xor E xor [0,SC[1]] xor [0xffffffff,0xffffff00];
+    Var E :: nil <:- E xor A xor [0,SC[2]] xor [0xffffffff,0xffffff00];
+    Var Ar :: Var Br :: Var Cr :: Var Dr :: Var Er :: nil <:- [D, C, A, E, B]
+tel.
+
+
+Definition node_ACE := node ACE args (input:u32x2[5]) returns (output:u32x2[5])
+vars
+    (SC:u32[3][16]) ::
+    (RC:u32[3][16]) ::
+    (tmp:u32x2[17][5]) :: nil
+let
+    Var SC :: nil <|- [0x50,0x5c,0x91,0x8d,0x53,0x60,0x68,0xe1,0xf6,0x9d,0x40,0x4f,0xbe,0x5b,0xe9,0x7f,
+          0x28,0xae,0x48,0xc6,0xa9,0x30,0x34,0x70,0x7b,0xce,0x20,0x27,0x5f,0xad,0x74,0x3f,
+          0x14,0x57,0x24,0x63,0x54,0x18,0x9a,0x38,0xbd,0x67,0x10,0x13,0x2f,0xd6,0xba,0x1f];
+    Var RC :: nil <|- [0x07,0x0a,0x9b,0xe0,0xd1,0x1a,0x22,0xf7,0x62,0x96,0x71,0xaa,0x2b,0xe9,0xcf,0xb7,
+          0x53,0x5d,0x49,0x7f,0xbe,0x1d,0x28,0x6c,0x82,0x47,0x6b,0x88,0xdc,0x8b,0x59,0xc6,
+          0x43,0xe4,0x5e,0xcc,0x32,0x4e,0x75,0x25,0xfd,0xf9,0x76,0xa0,0xb0,0x09,0x1e,0xad];
+
+    tmp[0] :: nil <|- input;
+
+    for i in 0 to 15 do
+        tmp[i+1] :: nil <|- ACE_step @ [tmp[i], RC $ [0,1,2][i],SC $ [0,1,2][i]]
+    done;
+
+    Var output :: nil <|- tmp[16]
+tel.
+
+Definition prog_ace_bs := node_ACE :: node_ACE_step :: node_simeck_box :: nil.
